

[TOC]

# Unit 3

## Inverse Matrix

- Only for square matrix

Let A be $n\times n$. The inverse of A is a matrix B satisfying the following properties

1. $AB=I_N$
2. $BA=I_N$

We denote it $B=A^{-1}$

### Example

$$
A=

\begin{bmatrix}
3 & 5\\
1 & 2
\end{bmatrix}\\
B=\begin{bmatrix}
2 & -5\\
-1 & 3
\end{bmatrix}\\\

AB=\begin{bmatrix}
3 & 5\\
1 & 2
\end{bmatrix}
\begin{bmatrix}
2 & -5\\
-1 & 3
\end{bmatrix}=
\begin{bmatrix}
1 & 0\\
0 & 1
\end{bmatrix}\\
BA=\begin{bmatrix}
2 & -5\\
-1 & 3
\end{bmatrix}
\begin{bmatrix}
3 & 5\\
1 & 2
\end{bmatrix}=
\begin{bmatrix}
1 & 0\\
0 & 1
\end{bmatrix}
$$

So $A^{-1} = \begin{bmatrix}
2 & -5\\
-1 & 3
\end{bmatrix}$ 

### General Formula

For $A\ 2\times 2$ matrix $A=\begin{bmatrix}
a & b\\
c & d
\end{bmatrix}$, the inverse is $A^{-1} = \frac{1}{ad-bc}\begin{bmatrix}
d & -b\\
-c & a
\end{bmatrix}$

The inverse exists provided that $ad-bc \neq 0$



Suppose $A^{-1}$ exists, where A is $n\times n$. 

- Consider $A\vec{x} = \vec{b}$
- Multiply by $A^{-1}$: $A^{-1}(A\vec{x}) = A^{-1}\vec{b}$ = $I_N\vec{x} = A^{-1}\vec{b}$
- $\vec{x} = A^{-1}\vec{b}$
- Therefore, if $A^{-1}$ exists then the system $A\vec{x} =\vec{b}$ has a unique solution which $\vec{x} = A^{-1}\vec{b}$ for any $\vec{b}$

### Theorem

The following statements are equivalent (all true or false) for $A$ that is $n\times n$:

- $A^{-1}$ exists
- $rank(A) = N$
- $A\vec{x} = \vec{b}$ Has a solution for all $\vec{b}$
- $A\vec{x} = \vec{0}$ Has only the trivial solution $\vec{x} = \vec{0}$
- The RREF of *A* is $I_N$



**Suppose** $A\vec{x} = \vec{b}$ has a solution for all $\vec{b}$. Let $\vec{b}_i$ be the $i-th$ column of the identity matrix. Let $\vec{c_i}$ be the solution of $A\vec{x} = \vec{b_i}$
$$
A=\begin{bmatrix}
1 & 1 & \dots & 1\\ 
\vec{C_1} & \vec{C_2} & \dots & \vec{C_N}\\
1 & 1 & \dots & 1\\
\end{bmatrix}=
\begin{bmatrix}
1 & 1 & \dots & 1\\ 
\vec{b_1} & \vec{b_2} & \dots & \vec{b_N}\\
1 & 1 & \dots & 1\\
\end{bmatrix}= I_N
$$

### To find $A^{-1}$:

$$
\begin{bmatrix}
A & | & I_N
\end{bmatrix}
$$

Reduce it to:
$$
\begin{bmatrix}
I_N & | & A^{-1}
\end{bmatrix}
$$


### Example

$$
A=

\begin{bmatrix}
1 & 1 & 1\\
1 & -1 & 0\\
1 & 0 & -1
\end{bmatrix}\\

\begin{bmatrix}
1 & 1 & 1 & | & 1 & 0 & 0\\
1 & -1 & 0 & | & 0 & 1 & 0\\
1 & 0 & -1 & | & 0 & 0 & 1
\end{bmatrix}=
\begin{bmatrix}
1 & 1 & 1 & | & 1 & 0 & 0\\
0 & -2 & -1 & | & -1 & 1 & 0\\
0 & -1 & -2 & | & -1 & 0 & 1
\end{bmatrix}=
\begin{bmatrix}
1 & 1 & 1 & | & 1 & 0 & 0\\
0 & -1 & -2 & | & -1 & 0 & 1\\
0 & 0 & 3 & | & 1 & 1 & -2
\end{bmatrix}=
\begin{bmatrix}
1 & 0 & 0 & | & \frac{1}{3} & \frac{1}{3} & \frac{1}{3}\\
0 & 1 & 0 & | & \frac{1}{3} & \frac{-2}{3} & \frac{1}{3}\\
0 & 0 & 1 & | & \frac{1}{3} & \frac{1}{3} & \frac{-2}{3}
\end{bmatrix}\\
A^{-1}= \frac{1}{3}
\begin{bmatrix}
1 & 1 & 1\\
1 & -2 & 1\\
1 & 1 & -2
\end{bmatrix}
$$



Recall $(AB)^T=B^TA^T$. Suppose $A^{-1}$ exists: $AA^{-1} = I_N$. 

Then $(AA^{-1})^T = (I_N)^T=I_N$.

Then $(A^{-1})^TA^T=I_N$

Therefore, $(A^T)^{-1} = (A^{-1})^T$



Note, if $A=A^T$ (i,e, $A$ is symmetric)

$(A^T)^{-1} = A^{-1} = (A^{-1})^T$

If *A* is symmetric, then $A^{-1}$

## Subspace

A subspace $W$ a set of vectors of $\R^N$ satisfying:

- $W$ Is closed under addition: if $\vec{v_1}$ and $\vec{v_2}$ are in $W$. Then $\vec{v_1}+\vec{v_2}$ is in $W$.
- $W$ Is closed under scalar products: if $\vec{v}$ is in $W$ and *a* is a scalar, then $a\vec{v}$ is in $W$

Note: $W$ is closed under linear combinations

Note: $\vec{0}$ is in every subspace

### Subspaces of $\R^2$

1. Each line through the origin is a subspace
2. $\{{\vec{0}}\}$ Is a subspace of $\R^N$ - trivial subspace
3. The whole space, $\R^2$, is also a subspace

### Theorem

$span(\vec{v_1},\vec{v_2},...,\vec{v_k})$ is a subspace